formalization/thesis/Isotope/LambdaSSA/Subtyping/Semantics.lean
@@ -1,0 +1,5 @@
+import Isotope.LambdaSSA.Subtyping.Semantics.Monadic.Term
+import Isotope.LambdaSSA.Subtyping.Semantics.Monadic.Region
+import Isotope.LambdaSSA.Subtyping.Semantics.Categorical.Term
+import Isotope.LambdaSSA.Subtyping.Semantics.Categorical.Region
+import Isotope.LambdaSSA.Subtyping.Semantics.Agreement.Term
