formalization/thesis/Isotope/LambdaSSA/Translation.lean
@@ -5,4 +5,6 @@ import Isotope.LambdaSSA.Translation.ANF.Elaboration.Semantics
 import Isotope.LambdaSSA.Translation.ANF.Elaboration.DirectElaborate
 import Isotope.LambdaSSA.Translation.ANF.ToSSA
 import Isotope.LambdaSSA.Translation.Compile
+import Isotope.LambdaSSA.Translation.Compile.Semantics
+import Isotope.LambdaSSA.Translation.Compile.Subtyping
 import Isotope.LambdaSSA.Translation.Frontend
