formalization/thesis/Isotope/LambdaSSA/Translation/Frontend.lean
@@ -1,3 +1,5 @@
 import Isotope.LambdaSSA.Translation.Frontend.NamedToLocallyNameless
 import Isotope.LambdaSSA.Translation.Frontend.LambdaCase
 import Isotope.LambdaSSA.Translation.Frontend.LambdaSeq
+import Isotope.LambdaSSA.Translation.Frontend.ExactSemantics
+import Isotope.LambdaSSA.Translation.Frontend.Subtyping
